tspmo

Aoc2025/Day01.lean
@@ -1,52 +1,99 @@
-abbrev Dial := Int
-def dialSize : Nat := 100
-def dialInit : Dial := 50
+namespace Day01
 
+abbrev dialSize : Int := 100
+structure Dial where
+  toInt : Int
+  isNormalised : toInt = toInt % dialSize
+
+def dialInit : Dial := ⟨50, by grind⟩
+
+theorem Dial.toInt_nonneg (d : Dial) : 0 <= d.toInt := by
+  rw [d.isNormalised]; grind
+
+/-- Note: DialState α over a monoid ⟨α, ×⟩ has the monoidal
+  structure ((×) <$> · <*> ·), which we will define
+  homomorphisms into. -/
 abbrev DialState α := StateM Dial α
 
 -- Rotate the dial by the given command.
 def stepDial (command : Int) : DialState Unit := do
   let dial <- get
-  set $ (dial + command) % dialSize
+  set $ Dial.mk ((dial.toInt + command) % dialSize) (by grind)
 
-theorem step_dial_homomorphism 
-  : ∀ c0 c1, stepDial (c0 + c1) = (do stepDial c0; stepDial c1) := by
-  intros
-  apply StateT.ext
-  intros
+/-- stepDial is a monoid homomorphism (ℤ, +) → DialState Unit. -/
+theorem stepDial_hom (c0 c1 : Int)
+  : stepDial (c0 + c1) = stepDial c0 *> stepDial c1 := by
+  intros; ext
   simp [stepDial]
   grind
 
+@[simp]
+theorem stepDial_zero : stepDial 0 = pure ⟨⟩ := by
+  ext d; simp [stepDial]; congr
+  rw [← d.isNormalised]
+
 -- Rotate the dial at once, only counting 0 at the end.
-def stepAtomic (command : Int) : DialState Int := do
+def stepAtomic (command : Int) : DialState Nat := do
   stepDial command
   let dial' <- get
-  return if dial' = 0 then 1 else 0
+  return if dial'.toInt = 0 then 1 else 0
 
 -- Rotate the dial one step at a time, counting every 0.
-def stepIncrementalSlow (command : Int) : DialState Int := do
-  let substates <- (List.replicate command.natAbs command.sign).mapM stepAtomic
-  return substates.sum
+def stepIncrementalSlow (command : Int) : DialState Nat :=
+  List.sum <$> (List.replicate command.natAbs command.sign).mapM stepAtomic
 
-def stepIncremental (command : Int) : DialState Int := do
+theorem Int.add_same_sign_eq (c0 c1 : Int)
+  : c0.sign = c1.sign →
+    (c0 + c1).sign = c1.sign := by
+  intro
+  if _ : c1 = 0
+  then grind [Int.eq_zero_of_sign_eq_zero]
+  else if _ : c1 > 0
+  then grind [Int.sign_eq_one_iff_pos]
+  else grind [Int.sign_eq_neg_one_iff_neg]
+
+theorem Int.natAbs_add_of_same_sign (c0 c1 : Int)
+  : c0.sign = c1.sign →
+    (c0 + c1).natAbs = c0.natAbs + c1.natAbs := by
+  intro
+  if _ : c1 = 0 then grind
+  else if _ : c1 > 0
+  then grind [Int.sign_eq_one_iff_pos, Int.natAbs_add_of_nonneg]
+  else grind [Int.sign_eq_neg_one_iff_neg, Int.natAbs_add_of_nonpos]
+
+/- stepIncrementalSlow is a monoid homomorphism
+ from the fixed-signed integers to DialState Nat. -/
+theorem stepIncrementalSlow_hom (c0 c1 : Int)
+  : c0.sign = c1.sign →
+    stepIncrementalSlow (c0 + c1)
+    = ((· + ·) <$> stepIncrementalSlow c0 <*> stepIncrementalSlow c1) := by
+  intros hsign; apply StateT.ext; intro dial0
+  simp [stepIncrementalSlow]
+  rw [Int.natAbs_add_of_same_sign _ _ hsign,
+       ← List.replicate_append_replicate, List.mapM_append,
+       Int.add_same_sign_eq _ _ hsign, hsign]
+  simp
+
+/- we could probably show that this is also a monoid homomorphism -/
+def stepIncremental (command : Int) : DialState Nat := do
   let dial <- get
   stepDial command
-  let rawDial' := dial + command
-  let mut fullRotations := rawDial'.natAbs / dialSize
-  if rawDial' <= 0 ∧ dial % dialSize != 0 then
+  let rawDial' := dial.toInt + command
+  let mut fullRotations := (rawDial'.natAbs / dialSize).natAbs
+  if rawDial' <= 0 ∧ dial.toInt != 0 then
     fullRotations := fullRotations + 1
   return fullRotations
 
 -- Run the stepping function over the commands.
-def runPart (step : Int -> DialState Int) (commands : Array Int) : Int :=
+def runPart (step : Int -> DialState Nat) (commands : Array Int) : Nat :=
   let allState := commands.mapM step
   let runAll := allState.run' dialInit
   runAll.sum
 
-def part1 (commands : Array Int) : Int :=
+def part1 (commands : Array Int) : Nat :=
   runPart stepAtomic commands
 
-def part2 (commands : Array Int) :=
+def part2 (commands : Array Int) : Nat :=
   runPart stepIncremental commands
 
 -- Read a line of input [LR]NNN as a rotation, L negative, R positive.
@@ -66,6 +113,9 @@ def parseInput : IO (Array Int) := do
   let lines <- stdin.lines
   let commands <- lines.mapM parseCommand
   return commands
+
+end Day01
+open Day01
 
 def main : IO Unit := do
   let commands <- parseInput
